src/ext_traversal/ExtTraversalProperties.v
@@ -1,0 +1,122 @@
+Require Import Setoid.
+From hahn Require Import Hahn.
+From imm Require Import Events Execution Execution_eco
+     TraversalConfig Traversal imm_common imm_s imm_s_hb CombRelations.
+Require Import AuxRel AuxRel2.
+Require Import ExtTraversal.
+
+Set Implicit Arguments.
+
+Section ExtTraversalProperties.
+Variable G : execution.
+Variable WF : Wf G.
+Variable COM : complete G.
+Variable sc : relation actid.
+Variable IMMCON : imm_consistent G sc.
+
+Notation "'acts'" := G.(acts).
+Notation "'sb'" := G.(sb).
+Notation "'rmw'" := G.(rmw).
+Notation "'data'" := G.(data).
+Notation "'addr'" := G.(addr).
+Notation "'ctrl'" := G.(ctrl).
+Notation "'rmw_dep'" := G.(rmw_dep).
+Notation "'rf'" := G.(rf).
+Notation "'co'" := G.(co).
+Notation "'coe'" := G.(coe).
+Notation "'fr'" := G.(fr).
+
+Notation "'eco'" := G.(eco).
+
+Notation "'bob'" := G.(bob).
+Notation "'fwbob'" := G.(fwbob).
+Notation "'ppo'" := G.(ppo).
+Notation "'fre'" := G.(fre).
+Notation "'rfi'" := G.(rfi).
+Notation "'rfe'" := G.(rfe).
+Notation "'deps'" := G.(deps).
+Notation "'detour'" := G.(detour).
+Notation "'release'" := G.(release).
+Notation "'sw'" := G.(sw).
+Notation "'hb'" := G.(hb).
+Notation "'rppo'" := G.(rppo).
+
+Notation "'urr'" := (urr G sc).
+Notation "'c_acq'" := (c_acq G sc).
+Notation "'c_cur'" := (c_cur G sc).
+Notation "'c_rel'" := (c_rel G sc).
+Notation "'t_acq'" := (t_acq G sc).
+Notation "'t_cur'" := (t_cur G sc).
+Notation "'t_rel'" := (t_rel G sc).
+Notation "'S_tm'" := G.(S_tm).
+Notation "'S_tmr'" := G.(S_tmr).
+Notation "'msg_rel'" := (msg_rel G sc).
+
+Notation "'lab'" := G.(lab).
+Notation "'loc'" := (loc lab).
+Notation "'val'" := (val lab).
+Notation "'mod'" := (Events.mod lab).
+Notation "'same_loc'" := (same_loc lab).
+
+Notation "'E'" := G.(acts_set).
+Notation "'R'" := (fun x => is_true (is_r lab x)).
+Notation "'W'" := (fun x => is_true (is_w lab x)).
+Notation "'F'" := (fun x => is_true (is_f lab x)).
+Notation "'RW'" := (R ∪₁ W).
+Notation "'FR'" := (F ∪₁ R).
+Notation "'FW'" := (F ∪₁ W).
+Notation "'R_ex'" := (fun a => is_true (R_ex lab a)).
+Notation "'W_ex'" := (W_ex G).
+Notation "'W_ex_acq'" := (W_ex ∩₁ (fun a => is_true (is_xacq lab a))).
+
+Notation "'Init'" := (fun a => is_true (is_init a)).
+Notation "'Loc_' l" := (fun x => loc x = Some l) (at level 1).
+Notation "'Tid_' t" := (fun x => tid x = t) (at level 1).
+Notation "'W_' l" := (W ∩₁ Loc_ l) (at level 1).
+
+Notation "'Pln'" := (fun x => is_true (is_only_pln lab x)).
+Notation "'Rlx'" := (fun x => is_true (is_rlx lab x)).
+Notation "'Rel'" := (fun x => is_true (is_rel lab x)).
+Notation "'Acq'" := (fun x => is_true (is_acq lab x)).
+Notation "'Acqrel'" := (fun x => is_true (is_acqrel lab x)).
+Notation "'Sc'" := (fun x => is_true (is_sc lab x)).
+Notation "'Acq/Rel'" := (fun a => is_true (is_ra lab a)).
+
+Variable T : ext_trav_config.
+Variable ETCCOH : etc_coherent G sc T.
+
+Notation "'S'" := (reserved T).
+Notation "'C'" := (ecovered T).
+Notation "'I'" := (eissued  T).
+
+Lemma rmw_in_rppo : rmw ⊆ rppo.
+Proof.
+  unfold ExtTraversal.rppo.
+  rewrite WF.(wf_rmwD).
+  rewrite WF.(rmw_in_sb).
+  basic_solver 10.
+Qed.
+
+Lemma rf_rmw_S : <|W_ex|> ;; rf ;; rmw ;; <|S|> ≡
+                 <|S|> ;; <| W_ex |> ;;  rf ;; rmw ;; <|S|>.
+Proof.
+  apply dom_rel_helper.
+  rewrite rfi_union_rfe, seq_union_l, seq_union_r, dom_union.
+  unionL.
+  { arewrite (rfi ⊆ sb). rewrite WF.(rmw_in_sb).
+    arewrite (sb ;; sb ⊆ sb).
+    { apply transitiveI. apply sb_trans. }
+    apply ETCCOH. }
+  arewrite_id ⦗W_ex⦘. rewrite seq_id_l.
+  rewrite rmw_in_rppo.
+  etransitivity.
+  2: by apply ETCCOH.(etc_I_in_S).
+  etransitivity.
+  2: by apply ETCCOH.(etc_rppo_S).
+  rewrite <- inclusion_id_rt, seq_id_l.
+  basic_solver 10.
+Qed.
+
+(* Lemma rf_rmw_S_rt *)
+
+End ExtTraversalProperties.
